學號：513717017 沈佩如

![image](https://github.com/user-attachments/assets/71aad8de-8683-4332-ad92-f059e347ba72)

$$Sxy=\frac{\left[\sum(XY)-\frac{(\sum X)(\sum Y)}{n}\right]}{n-1}=\frac{\left[4558-\frac{(266)(169)}{10}\right]}{9}=6.96$$

$$Sx^2 = \frac{\left[\sum(X^2) - \frac{(\sum X)^2}{n}\right]}{n-1} =  \frac{\left[(7230) - \frac{(266)^2}{10}\right]}{9}= 17.16$$

$$Sx = \sqrt{Sx^2} = \sqrt{17.16}=4.14$$

$$Sy^2 = \frac{\left[\sum(Y^2) - \frac{(\sum Y)^2}{n}\right]}{n-1}  = \frac{\left[\(2887) - \frac{(169)^2}{10}\right]}{9} = 3.43$$

$$Sy = \sqrt{Sy^2} = \sqrt{3.43}=1.85$$

$$ r=\frac{Sxy}{Sx Sy}=\frac{6.96}{4.14*1.85}=0.91$$
