![image](https://github.com/user-attachments/assets/cf68f5df-1daa-404d-a24a-e2068965413e)

a. 

$p(1)=(1-\frac{1}{10})^{1-1}\times\frac{1}{10}=1\times\frac{1}{10}=\frac{1}{10}$

$p(2)=(1-\frac{1}{10})^{2-1}\times\frac{1}{10}=\frac{9}{10}\times\frac{1}{10}=\frac{9}{100}$

$p(3)=(1-\frac{1}{10})^{3-1}\times\frac{1}{10}=(\frac{9}{10})^2\times\frac{1}{10}=\frac{81}{1000}$

b.

$p(x)=(1-\frac{1}{10})^{x-1}\times\frac{1}{10}$

c.

![image](https://github.com/user-attachments/assets/5ce71d2f-0b4b-43bb-a46f-beb3d87309f0)
